

Karush - Kuhn - Tucker Conditions:

$$\min_x f(x)$$

x is a $n \times 1$ vector on real numbers
 $x \in \mathbb{R}^n$

$$\text{Subj. to } l_j(x) = 0, \quad j=1, \dots, r$$

$$h_i(x) \leq 0, \quad i=1, \dots, m$$

Optimality Conditions

We define the Lagrangian as

$$\begin{aligned} L(x, \lambda, \mu) &= f(x) + \sum_{j=1}^r \lambda_j l_j(x) + \sum_{i=1}^m \mu_i h_i(x) \\ &= f(x) + \sum_{j=1}^r \lambda_j l_j(x) + \sum_{i=1}^m \mu_i h_i(x) \end{aligned}$$

The necessary conditions of optimality are called KKT conditions. They are as follows:

$$\bullet \quad \frac{\partial L}{\partial x_k} = \frac{\partial f(x)}{\partial x_k} + \sum_{j=1}^r \lambda_j \frac{\partial l_j(x)}{\partial x_k} + \sum_{i=1}^m \mu_i \frac{\partial h_i(x)}{\partial x_k} = 0$$

$$k \in (1, 2, \dots, n)$$

$$\bullet \quad l_j(x) = 0, \quad h_i(x) \leq 0 \quad \text{for all } i, j$$

$$\bullet \quad \mu_i h_i(x) = 0 \quad \text{for all } i$$

$$\bullet \quad \mu_i \geq 0 \quad \text{for all } i$$

Example 1

$$\text{Minimize } f = x_1^2 + 2x_2^2 + 3x_3^2$$

$$g_1 = x_1 - x_2 - 2x_3 \leq 12$$

$$g_2 = x_1 + 2x_2 - 3x_3 \leq 8$$

Using KKT conditions

$$\begin{aligned} \text{Solution } L &= (x_1^2 + 2x_2^2 + 3x_3^2) + \mu_1 (x_1 - x_2 - 2x_3 - 12) \\ &\quad + \mu_2 (x_1 + 2x_2 - 3x_3 - 8) \end{aligned}$$

$$\frac{\partial L}{\partial x_1} = 2x_1 + \mu_1 + \mu_2 = 0 \quad \text{--- (1)}$$

$$\frac{\partial L}{\partial x_2} = 4x_2 - \mu_1 + 2\mu_2 = 0 \quad \text{--- (2)}$$

$$\frac{\partial L}{\partial x_3} = 6x_3 - 2\mu_1 - 3\mu_2 = 0 \quad \text{--- (3)}$$

$$\mu_1 (x_1 - x_2 - 2x_3 - 12) = 0 \quad \text{--- (4)}$$

$$\mu_2 (x_1 + 2x_2 - 3x_3 - 8) = 0 \quad \text{--- (5)}$$

$$x_1 - x_2 - 2x_3 - 12 \leq 0 \quad \text{--- (6)}$$

$$x_1 + 2x_2 - 3x_3 - 8 \leq 0 \quad \text{--- (7)}$$

$$\mu_1 \geq 0, \mu_2 \geq 0 \quad \text{--- (8)}$$

Case I:

$$\mu_1 = 0$$

putting $\mu_1 = 0$ in (1), (2), (3)

$$x_1 = x_2 = -\frac{\mu_2}{2}, \quad x_3 = \frac{\mu_2}{2}$$

Sub write eq (5),

$$\mu_2 \left(-\frac{\mu_2}{2} - \frac{2\mu_2}{2} - 3 \cdot \frac{\mu_2}{2} - 8 \right) = 0$$

$$-3\mu_2^2 - 8\mu_2 = 0$$

$$\therefore \mu_2 = 0 \text{ or } -\frac{8}{3}$$

$$\Rightarrow \mu_2 = 0 \rightarrow X^* = [0, 0, 0]$$

Case II:

$$x_1 - x_2 - 2x_3 - 12 = 0$$

$$\text{or, } -\frac{(\mu_1 + \mu_2)}{2} - \frac{(\mu_1 - 2\mu_2)}{4} - \frac{2\mu_1 + 3\mu_2}{3} - 12 = 0$$

$$\text{or, } 17\mu_1 + 12\mu_2 = -144 \quad \text{--- inconsistent with}$$

$$\mu_1 \geq 0, \mu_2 \geq 0$$

$$\therefore \text{Solution is } [0 \ 0 \ 0]^T$$